Use Arguments _ : efault implicits for Codes, Terms

sandbox/Compile.v
@@ -3,9 +3,6 @@ Require Import Combinators.
 Require Import DeBruijn.
 Require Import BohmTrees.
 
-Definition protect {Var : Set} : Term Var -> Term (option' Var) :=
-  term_map (@Some Var).
-
 Fixpoint compile {Var : Set} (t : Term Var) : Code Var :=
   match t with
   | TOP%term => TOP%code
@@ -16,6 +13,50 @@ Fixpoint compile {Var : Set} (t : Term Var) : Code Var :=
   | term_var v => code_var v
   | term_lambda x => code_abs id (compile x)
   end.
+
+Inductive compiles_to {Var : Set} : Term Var -> Code Var -> Prop :=
+  | compiles_to_top : compiles_to TOP%term TOP%code
+  | compiles_to_bot : compiles_to BOT%term BOT%code
+  | compiles_to_join x x' y y' :
+     compiles_to x x' -> compiles_to y y' ->
+     compiles_to (x || y) (x' || y')%code
+  | compiles_to_rand x x' y y' :
+     compiles_to x x' -> compiles_to y y' ->
+     compiles_to (x (+) y) (x' (+) y')%code
+  | compiles_to_app x x' y y' :
+     compiles_to x x' -> compiles_to y y' ->
+     compiles_to (x * y) (x' * y')%code
+  | compiles_to_var v : compiles_to (term_var v) (code_var v)
+  | compiles_to_lambda x x' :
+      @compiles_to (option Var) x x' ->
+      compiles_to (term_lambda x) (code_abs id x')
+.
+Hint Constructors compiles_to.
+
+Section compiles_to_compile.
+  Local Ltac compiles_to_compiles :=
+    simpl;
+    repeat match goal with
+    | [ H' : forall c : _, compiles_to ?t c -> compile ?t = c |- _] =>
+      match goal with
+      | [ H : compiles_to ?t ?c' |- _] =>
+        apply H' in H; rewrite H; clear H; simpl
+      end
+    end;
+    auto.
+
+  Lemma compiles_to_compile (Var : Set) (t : Term Var) (c : Code Var) :
+    compiles_to t c <-> compile t = c.
+  Proof.
+    split.
+    - intro H; induction t; inversion H; compiles_to_compiles.
+    - intro H; induction t; simpl in H; rewrite <- H; auto.
+  Qed.
+End compiles_to_compile.
+
+
+Definition protect {Var : Set} : Term Var -> Term (option' Var) :=
+  term_map (@Some Var).
 
 (* TODO this needs to be changed to get [decompile_compile] to hold,
    at least when restricted to Bohm trees. *)
@@ -46,7 +87,7 @@ Fixpoint decompile {Var : Set} (c : Code Var) : Term Var :=
       let x' := protect (decompile x) in
       let y' := protect (decompile y) in
       let v := VAR None in
-      LAMBDA (x' * v * y')
+      LAMBDA (x' * v * (y' * v))
   | (x * y)%code => (decompile x * decompile y)
   | code_var v => term_var v
   (* these cases never arise as [decompile (compile t)] *)
@@ -58,17 +99,32 @@ Fixpoint decompile {Var : Set} (c : Code Var) : Term Var :=
   | R => DeBruijn.K (+) DeBruijn.F
   end.
 
-(* maybe restrict [t] to Bohm trees *)
-Lemma decompile_compile (Var : Set) (t : Term Var) : decompile (compile t) = t.
-Proof.
-  induction t; simpl; auto.
-  - rewrite IHt1, IHt2; reflexivity.
-  - rewrite IHt1, IHt2; reflexivity.
-  - rewrite IHt1, IHt2; clear IHt1 IHt2.
-    case_eq t1; simpl; auto.
-    + intros; case_eq (compile t); auto;
+
+Section decompile_compile.
+  Local Ltac decompile_compile :=
+    simpl;
+    repeat match goal with
+    | [H : decompile (compile ?x) = ?x |- _] => rewrite H; clear H; simpl
+    end.
+
+  Lemma decompile_compile_normal (Var : Set) (t : Term Var) :
+   normal t -> decompile (compile t) = t.
+  Proof.
+    intro Hn; induction Hn; decompile_compile; auto.
+    - case_eq (compile x); intros; try (compute; reflexivity);
       admit.
-    + intros; case_eq (code_abs id (compile t)); intros; subst; auto;
-      admit.
-  - admit.
-Qed.
+    - admit.
+  Qed.
+
+  Lemma decompile_compile (Var : Set) (t : Term Var) :
+    decompile (compile t) = t.
+  Proof.
+    induction t; decompile_compile; auto.
+    - case_eq (compile t1); simpl; auto.
+      + intros; case_eq c; auto;
+        admit.
+      + intros.
+        admit.
+    - admit.
+  Qed.
+End decompile_compile.
